some more experiments on type quotation

SailLean/Syntax/Quote.lean
@@ -3,32 +3,74 @@ import SailLean.Syntax.Elab
 import Aesop
 import Qq
 
-open Qq
+open Qq Lean Elab Term
 
 namespace Sail
 
-inductive TypArg where | nexp (n : Q(Nat)) | type (t : Q(Type)) | bool (c : Q(Prop))
+/-inductive TypArg where | nexp (n : Q(Nat)) | type (t : Q(Type)) | bool (c : Q(Prop))
+  deriving Repr-/
 
-def quoteTypArgType : TypArg → Q(Type)
-  | .nexp n => q(Unit)  -- TODO quote as equality somehow
-  | .type t => t
-  | .bool c => q(Inhabited $c)  -- TODO sure?
+/-- Obtain the kind of a typ argument. -/
+def AST.TypArg.kind : AST.TypArg → AST.Kind
+  | .nexp _ => .int
+  | .bool _ => .bool
+  | .typ _ => .type
 
-def liftListToProduct : List Q(Type) → Q(Type)
-  | [] => q(Unit)
+/-- Quote Sail's type parameter into `Type 1` (instead of `Type`, since they can be quoted to
+`Type`s) -/
+def quoteKind : AST.Kind → Q(Type 1)
+  | .int => q(ULift Nat)
+  | .bool => q(ULift Prop)
+  | .type => q(Type)
+
+def quoteTypArg : (a : AST.TypArg) → Q($(quoteKind a.kind))
+  | .nexp n => q(⟨42⟩)  -- TODO quote as equality somehow
+  | .typ t => q(Unit)  -- TODO need recursion here
+  | .bool c => q(⟨True⟩)  -- TODO quote nconstraints
+
+def liftListToProduct : List Q(Type) → Q(Type 1)
+  | [] => q(PUnit.{2})
   | [t] => t
   | t::ts => q($t × $(liftListToProduct ts))
 
-def liftTypArgListToProduct : List TypArg → Q(Type) :=
-  liftListToProduct ∘ (·.map quoteTypArgType)
+def liftKindListToProduct : List AST.Kind → Q(Type 1) :=
+  liftListToProduct ∘ (·.map quoteKind)
 
-def RegisteredTypeKind : List TypArg → Type
-  | [] => Q(Type)
-  | args@(_::_) => Q(Type → Type)
+/-- Build a tuple -/
+def buildTuple (ts : List Expr) (es : List Expr) : Expr :=
+ match ts, es with
+ | [], [] => (q(.unit) : Q(PUnit.{2}))
+ | [_], [e] => e
+ | (t::ts), (e::es) => mkApp4 (.const `Prod.mk [mkLevelSucc levelOne]) t (liftListToProduct ts) e (buildTuple ts es)
+ | _, _ => panic! "incorrect number of arguments!"
+
+/-- Build the tuple of type arguments given a `List AST.TypArg`.
+It should have the type `liftKindListToProduct (args.map AST.TypArg.kind)`. -/
+def liftTypArgListToTuple (args : List AST.TypArg) :
+    Q($(liftKindListToProduct (args.map AST.TypArg.kind))) :=
+  buildTuple (args.map (quoteKind ∘ AST.TypArg.kind)) (args.map quoteTypArg)
+
+def RegisteredTypeKind : List AST.Kind → Q(Type 1)
+  | [] => q(Type)
+  | args@(_::_) => q($(liftKindListToProduct args) → Type)
+
+@[simp]
+theorem registeredTypeKind_nil : RegisteredTypeKind [] = q(Type) := rfl
+
+@[simp]
+theorem registeredTypeKind_cons :
+     RegisteredTypeKind (a::as) = q($(liftKindListToProduct (a::as)) → Type) := rfl
 
 structure RegisteredType where
-  args : List TypArg := []
-  type : RegisteredTypeKind args
+  params : List AST.Kind := []
+  type : Q($(RegisteredTypeKind params))
+
+instance : Repr RegisteredType where
+  reprPrec o _ :=
+    match o with
+    | ⟨params@ [], t⟩
+    | ⟨params@ (_::_), t⟩ =>
+      s!"({repr params}, {by { simp at t; exact repr t }})"
 
 structure Env where
   typ_ids : Std.HashMap AST.Id RegisteredType
@@ -40,24 +82,46 @@ def sailBool : RegisteredType where
   type := q(_root_.Bool)
 
 def sailFin : RegisteredType where
-  args := [.type q(Nat)]
-  type := q(Fin)
+  params := [.int]
+  type := q(Fin ∘ ULift.down)  -- TODO see if the `ulift`s are getting too annoying to work with
+
+def foo : List α → _root_.Bool
+  | [] => .false
+  | (_::_) => .true
 
 def std_env : Env where
-  typ_ids := Std.HashMap.ofList [(.ident `bool, sailBool), (.ident `fin, sailFin)]
+  typ_ids := Std.HashMap.ofList
+    [(.ident "bool", sailBool)
+     , (.ident "fin", sailFin)]
 
-partial def quoteTyp (e : Env) : AST.Typ → Q(Type)
-  | .fn []          dom => quoteTyp e dom
-  | .fn args       dom => q($(liftListToProduct (args.map (quoteTyp e))) → $(quoteTyp e dom))
-  | .tuple []      => q(Unit)
+/-- Quotes any Typ from the AST into the quotation of a Lean type, provided an environment -/
+partial def quoteTyp (e : Env) : AST.Typ → Lean.Elab.Term.TermElabM Q(Type 1)
+  | .fn []         dom => quoteTyp e dom
+  | .fn args       dom => return q($(liftListToProduct (← args.mapM (quoteTyp e)))
+                                      → $(← quoteTyp e dom))
+  | .tuple []      => return q(PUnit)
   | .tuple [t]     => quoteTyp e t
-  | .tuple (t::ts) => q($(quoteTyp e t) × $(quoteTyp e (.tuple ts)))
-  | .id i =>
-      let ⟨args, t⟩ := e.typ_ids.getD i sailUnit  -- TODO fail instead
-      match args with
-      | [] => t
-      | _ => panic! "called type without giving arguments"  -- TODO tidy
-  | _ => q(Unit)
+  | .tuple (t::ts) => return q($(← quoteTyp e t) × $(← quoteTyp e (.tuple ts)))
+  | .app i args =>
+      --println! "fgoo"
+      match e.typ_ids[i]? with
+      | .some ⟨params, t⟩ =>
+        match params with
+        | [] => return t
+        | params@(_::_) => do
+          let argTuple := liftTypArgListToTuple args
+          unless params = args.map AST.TypArg.kind do
+            panic! "kind of argument do not match the kinds of parameters!"
+          let e := mkApp t argTuple
+          return e
+      | _ => throwError "could not find type {repr i} in environment. \n
+         environment: {repr e.typ_ids.toList}"
+  | _ => throwError "unable to quote type"
 
-#eval! Lean.Meta.ppExpr <| quoteTyp std_env <|
-  (.tuple [.tuple [], .fn [.id (.ident `bool)] (.tuple [])])
+def testTypeQuotation (stx : Lean.Elab.Term.TermElabM (Lean.TSyntax `typ)) :
+    Lean.Elab.Term.TermElabM Lean.Format := do
+  let .ok astx := elabTyp (← stx) | throwError "unable to elaborate type"
+  let qt ← quoteTyp std_env astx
+  Lean.Meta.ppExpr qt
+
+#eval testTypeQuotation `(typ|(foo))
